utp/examples/find_replace.thy
@@ -6,31 +6,36 @@ begin
 
 utp_lit_vars
 
-alphabet ss = 
-  arr :: "nat \<Rightarrow> string"
-  occ :: "nat"
-  i   :: "nat"
+alphabet ss = arr::"nat \<Rightarrow> string" occ::"nat" i::"nat"
 
 definition find_replace :: 
   "(nat \<Rightarrow> string) \<Rightarrow> nat \<Rightarrow> string \<Rightarrow> string \<Rightarrow> ss hrel" where
-"find_replace inp len mtc rpl =
-  arr := inp ;; i := 0 ;; occ := 0 ;;
+"find_replace A len mtc rpl =
+  arr := A ;; i := 0 ;; occ := 0 ;;
   while i < len 
-  invr arr = (\<lambda> k. if k < i \<and> inp k = mtc then rpl else inp k)
-     \<and> occ = length (filter ((=) mtc) (map inp [0..<i]))
+  invr arr = (\<lambda> k. if k < i \<and> A k = mtc then rpl else A k)
+     \<and> occ = length (filter ((=) mtc) (map A [0..<i])) \<and> i \<le> len
   do
-    if (arr i = mtc)
-    then arr[i] := rpl ;; occ := occ + 1
+    if (arr i = mtc) then arr[i] := rpl ;; occ := occ + 1
     else arr[i] := arr i
-    fi ;;
-    i := i + 1
+    fi ;; i := i + 1
   od"    
 
-lemma find_replace_correct:
+lemma find_replace_inv:
   "\<^bold>{true\<^bold>}
-    find_replace inp len mtc rpl
-   \<^bold>{arr = (\<lambda> k. if k < i \<and> inp k = mtc then rpl else inp k)\<^bold>}"
+    find_replace A len mtc rpl
+   \<^bold>{arr = (\<lambda> k. if k < i \<and> A k = mtc then rpl else A k)\<^bold>}"
   unfolding find_replace_def
   by (hoare_split, rel_auto', metis less_Suc_eq)
+
+lemma find_replace_prop1:
+  "\<^bold>{true\<^bold>} find_replace A len mtc rpl \<^bold>{\<forall> i < len. A(i) = mtc \<Rightarrow> arr(i) = rpl\<^bold>}"
+  unfolding find_replace_def by (hoare_auto, metis less_Suc_eq)
+  
+lemma find_replace_prop2:
+  "\<^bold>{true\<^bold>} find_replace A len mtc rpl \<^bold>{occ = length (filter ((=) mtc) (map A [0..<len]))\<^bold>}"
+  unfolding find_replace_def by (hoare_auto, metis less_Suc_eq)
+
+
 
 end
